MathematicalLogic/FirstOrder/Bounded.lean
@@ -11,18 +11,18 @@ inductive BTerms (𝓛 : Language) (m : ℕ) : ℕ → Type where
 | cons : BTerm 𝓛 m → BTerms 𝓛 m n → BTerms 𝓛 m (n + 1)
 end
 
-prefix:max "#'" => BTerm.var
-infix:70 " ⬝ₜ " => BTerm.func
-notation "[]ₜ" => BTerms.nil
-infixr:75 " ∷ₜ " => BTerms.cons
+prefix:max "#ᵇ" => BTerm.var
+infix:70 " ⬝ₜᵇ " => BTerm.func
+notation "[]ₜᵇ" => BTerms.nil
+infixr:75 " ∷ₜᵇ " => BTerms.cons
 
 mutual
 @[simp] def BTerm.size : BTerm 𝓛 m → ℕ
-| #'_ => 0
-| _ ⬝ₜ ts => ts.size + 1
+| #ᵇ_ => 0
+| _ ⬝ₜᵇ ts => ts.size + 1
 @[simp] def BTerms.size : BTerms 𝓛 m n → ℕ
-| []ₜ => 0
-| t ∷ₜ ts => t.size + ts.size + 1
+| []ₜᵇ => 0
+| t ∷ₜᵇ ts => t.size + ts.size + 1
 end
 termination_by
   BTerm.size t => sizeOf t
@@ -35,20 +35,20 @@ instance (priority := high) : SizeOf (BTerms 𝓛 m n) := ⟨BTerms.size⟩
 
 mutual
 def BTerm.unbounded : BTerm 𝓛 m → Term 𝓛
-| #'x => #x
-| f ⬝ₜ ts => f ⬝ₜ ts.unbounded
+| #ᵇx => #x
+| f ⬝ₜᵇ ts => f ⬝ₜ ts.unbounded
 def BTerms.unbounded : BTerms 𝓛 m n → Terms 𝓛 n
-| []ₜ => []ₜ
-| t ∷ₜ ts => t.unbounded ∷ₜ ts.unbounded
+| []ₜᵇ => []ₜ
+| t ∷ₜᵇ ts => t.unbounded ∷ₜ ts.unbounded
 end
 
-@[simp] theorem BTerm.unbounded_var : (#'x : BTerm 𝓛 m).unbounded = #x := by simp [BTerm.unbounded]
-@[simp] theorem BTerm.unbounded_func : (f ⬝ₜ ts : BTerm 𝓛 m).unbounded = f ⬝ₜ ts.unbounded := by simp [BTerm.unbounded]
-@[simp] theorem BTerms.unbounded_nil : ([]ₜ : BTerms 𝓛 m 0).unbounded = ([]ₜ : Terms 𝓛 0) := rfl
-@[simp] theorem BTerms.unbounded_cons : (t ∷ₜ ts : BTerms 𝓛 m _).unbounded = t.unbounded ∷ₜ ts.unbounded := by simp [BTerms.unbounded]
+@[simp] theorem BTerm.unbounded_var : (#ᵇx : BTerm 𝓛 m).unbounded = #x := by simp [BTerm.unbounded]
+@[simp] theorem BTerm.unbounded_func : (f ⬝ₜᵇ ts : BTerm 𝓛 m).unbounded = f ⬝ₜ ts.unbounded := by simp [BTerm.unbounded]
+@[simp] theorem BTerms.unbounded_nil : ([]ₜᵇ : BTerms 𝓛 m 0).unbounded = ([]ₜ : Terms 𝓛 0) := rfl
+@[simp] theorem BTerms.unbounded_cons : (t ∷ₜᵇ ts : BTerms 𝓛 m _).unbounded = t.unbounded ∷ₜ ts.unbounded := by simp [BTerms.unbounded]
 
--- instance : CoeOut (BTerm 𝓛 m) (Term 𝓛) := ⟨BTerm.unbounded⟩
--- instance : CoeOut (BTerms 𝓛 m n) (Terms 𝓛 n) := ⟨BTerms.unbounded⟩
+instance : CoeOut (BTerm 𝓛 m) (Term 𝓛) := ⟨BTerm.unbounded⟩
+instance : CoeOut (BTerms 𝓛 m n) (Terms 𝓛 n) := ⟨BTerms.unbounded⟩
 
 mutual
 @[simp] def Term.bound : Term 𝓛 → ℕ
@@ -62,12 +62,12 @@ end
 mutual
 @[simp] def Term.bounded :
   (t : Term 𝓛) → m ≥ t.bound → BTerm 𝓛 m
-| #x, h => #'⟨x, by simp at h; exact h⟩
-| f ⬝ₜ ts, h => f ⬝ₜ ts.bounded (by simp at h; exact h)
+| #x, h => #ᵇ⟨x, by simp at h; exact h⟩
+| f ⬝ₜ ts, h => f ⬝ₜᵇ ts.bounded (by simp at h; exact h)
 @[simp] def Terms.bounded :
   (ts : Terms 𝓛 n) → m ≥ ts.bound → BTerms 𝓛 m n
-| []ₜ, _ => []ₜ
-| t ∷ₜ ts, h => t.bounded (by simp at h; exact h.left) ∷ₜ ts.bounded (by simp at h; exact h.right)
+| []ₜ, _ => []ₜᵇ
+| t ∷ₜ ts, h => t.bounded (by simp at h; exact h.left) ∷ₜᵇ ts.bounded (by simp at h; exact h.right)
 end
 
 mutual
@@ -90,58 +90,67 @@ def BSubst (𝓛 m k) := Fin m → BTerm 𝓛 k
 
 mutual
 def BTerm.subst : BTerm 𝓛 m → BSubst 𝓛 m k → BTerm 𝓛 k
-| #'x, σ => σ x
-| f ⬝ₜ ts, σ => f ⬝ₜ ts.subst σ
+| #ᵇx, σ => σ x
+| f ⬝ₜᵇ ts, σ => f ⬝ₜᵇ ts.subst σ
 def BTerms.subst : BTerms 𝓛 m n → BSubst 𝓛 m k → BTerms 𝓛 k n
-| []ₜ, σ => []ₜ
-| t ∷ₜ ts, σ => t.subst σ ∷ₜ ts.subst σ
+| []ₜᵇ, σ => []ₜᵇ
+| t ∷ₜᵇ ts, σ => t.subst σ ∷ₜᵇ ts.subst σ
 end
 
-notation:80 t "[" σ "]ₜ" => BTerm.subst t σ
-notation:80 ts "[" σ "]ₜₛ" => BTerms.subst ts σ
+notation:80 t "[" σ "]ₜᵇ" => BTerm.subst t σ
+notation:80 ts "[" σ "]ₜₛᵇ" => BTerms.subst ts σ
 
-@[simp] theorem BTerm.subst_var : (#'x : BTerm 𝓛 m)[σ]ₜ = σ x := by simp [BTerm.subst]
-@[simp] theorem BTerm.subst_func : (f ⬝ₜ ts : BTerm 𝓛 m)[σ]ₜ = f ⬝ₜ ts[σ]ₜₛ := by simp [BTerm.subst]
-@[simp] theorem BTerms.subst_nil {σ : BSubst 𝓛 m k} : ([]ₜ)[σ]ₜₛ = ([]ₜ : BTerms 𝓛 k 0) := by simp [BTerms.subst]
-@[simp] theorem BTerms.subst_cons : (t ∷ₜ ts : BTerms 𝓛 m _)[σ]ₜₛ = t[σ]ₜ ∷ₜ ts[σ]ₜₛ := by simp [BTerms.subst]
+@[simp] theorem BTerm.subst_var : (#ᵇx)[σ]ₜᵇ = σ x := by simp [BTerm.subst]
+@[simp] theorem BTerm.subst_func : (f ⬝ₜᵇ ts)[σ]ₜᵇ = f ⬝ₜᵇ ts[σ]ₜₛᵇ := by simp [BTerm.subst]
+@[simp] theorem BTerms.subst_nil {σ : BSubst 𝓛 m k} : ([]ₜᵇ)[σ]ₜₛᵇ = []ₜᵇ := by simp [BTerms.subst]
+@[simp] theorem BTerms.subst_cons : (t ∷ₜᵇ ts : BTerms 𝓛 m _)[σ]ₜₛᵇ = t[σ]ₜᵇ ∷ₜᵇ ts[σ]ₜₛᵇ := by simp [BTerms.subst]
 
-def BSubst.id : BSubst 𝓛 m m := λ x => #'x
-notation "idₛ" => BSubst.id
+def BSubst.id : BSubst 𝓛 m m := λ x => #ᵇx
+notation "idᵇ" => BSubst.id
 
 mutual
-theorem BTerm.subst_id {t : BTerm 𝓛 m} : t[idₛ]ₜ = t :=
+theorem BTerm.subst_id : t[idᵇ]ₜᵇ = t :=
   match t with
-  | #'x => by simp [BSubst.id]
-  | f ⬝ₜ ts => by simp; apply BTerms.subst_id
-theorem BTerms.subst_id {ts : BTerms 𝓛 m n} : ts[idₛ]ₜₛ = ts :=
+  | #ᵇx => by simp [BSubst.id]
+  | f ⬝ₜᵇ ts => by simp; apply BTerms.subst_id
+theorem BTerms.subst_id {ts : BTerms 𝓛 m n} : ts[idᵇ]ₜₛᵇ = ts :=
   match ts with
-  | []ₜ => rfl
-  | t ∷ₜ ts => by simp; rw [BTerm.subst_id, BTerms.subst_id]; trivial
+  | []ₜᵇ => rfl
+  | t ∷ₜᵇ ts => by simp; rw [BTerm.subst_id, BTerms.subst_id]; trivial
 end
 
-def BSubst.shift : BSubst 𝓛 m (m + 1) := λ x => #'(Fin.succ x)
-def BTerm.shift (t : BTerm 𝓛 m) := t[BSubst.shift]ₜ
-prefix:max "↑ₜ" => BTerm.shift
+def BSubst.nil : BSubst 𝓛 0 m := Fin.elim0
+notation "εᵇ" => BSubst.nil
 
-def BSubst.single (t : BTerm 𝓛 m) : BSubst 𝓛 (m + 1) m := Fin.cons t id
-prefix:max "↦ₛ " => BSubst.single
+def BSubst.cons (t : BTerm 𝓛 m) (σ : BSubst 𝓛 n m) : BSubst 𝓛 (n + 1) m :=
+  Fin.cons t σ
+infix:60 " ∷ₛᵇ " => BSubst.cons
 
-def BSubst.lift (σ : BSubst 𝓛 m k) : BSubst 𝓛 (m + 1) (k + 1) := Fin.cons #'0 (λ x => ↑ₜ(σ x))
-prefix:max "⇑ₛ" => BSubst.lift
+def BSubst.shift : BSubst 𝓛 m (m + 1) := λ x => #ᵇ(Fin.succ x)
+def BTerm.shift (t : BTerm 𝓛 m) := t[BSubst.shift]ₜᵇ
+prefix:max "↑ₜᵇ" => BTerm.shift
+
+def BSubst.single (t : BTerm 𝓛 m) : BSubst 𝓛 (m + 1) m :=
+  t ∷ₛᵇ id
+prefix:max "↦ᵇ " => BSubst.single
+
+def BSubst.lift (σ : BSubst 𝓛 m k) : BSubst 𝓛 (m + 1) (k + 1) :=
+  #ᵇ0 ∷ₛᵇ (λ x => ↑ₜᵇ(σ x))
+prefix:max "⇑ᵇ" => BSubst.lift
 
 mutual
 theorem BTerm.unbounded_subst_eq
   {t : BTerm 𝓛 m} {σ : BSubst 𝓛 m k} {σ' : Subst 𝓛} :
-  (∀ x, (σ x).unbounded = σ' x) → t[σ]ₜ.unbounded = t.unbounded[σ']ₜ :=
+  (∀ x, σ x = σ' x) → t[σ]ₜᵇ = t[σ']ₜ :=
   match t with
-  | #'x => by intro h; simp [h]
-  | f ⬝ₜ ts => by intro h; simp; exact BTerms.unbounded_subst_eq h
+  | #ᵇx => by intro h; simp [h]
+  | f ⬝ₜᵇ ts => by intro h; simp; exact BTerms.unbounded_subst_eq h
 theorem BTerms.unbounded_subst_eq
   {ts : BTerms 𝓛 m n} {σ : BSubst 𝓛 m k} {σ' : Subst 𝓛} :
-  (∀ x, (σ x).unbounded = σ' x) → ts[σ]ₜₛ.unbounded = ts.unbounded[σ']ₜₛ :=
+  (∀ x, σ x = σ' x) → (ts[σ]ₜₛᵇ : Terms 𝓛 n) = ts[σ']ₜₛ :=
   match ts with
-  | []ₜ => by intro; rfl
-  | t ∷ₜ ts => by
+  | []ₜᵇ => by intro; rfl
+  | t ∷ₜᵇ ts => by
     intro h
     simp
     rw [BTerm.unbounded_subst_eq h, BTerms.unbounded_subst_eq h]
@@ -149,7 +158,7 @@ theorem BTerms.unbounded_subst_eq
 end
 
 theorem BTerm.unbounded_shift_eq {t : BTerm 𝓛 m} :
-  t.shift.unbounded = t.unbounded.shift := by
+  ↑ₜᵇt = ↑ₜ(t : Term 𝓛) := by
   simp [BTerm.shift, Term.shift]
   apply BTerm.unbounded_subst_eq
   intro x
@@ -163,7 +172,7 @@ inductive BFormula (𝓛 : Language) : ℕ → Type where
 | imp : BFormula 𝓛 m → BFormula 𝓛 m → BFormula 𝓛 m
 | all : BFormula 𝓛 (m + 1) → BFormula 𝓛 m
 
-infix:70 " ⬝ₚ " => BFormula.atom
+infix:70 " ⬝ₚᵇ " => BFormula.atom
 instance : FormulaSymbol (BFormula 𝓛 m) := ⟨BFormula.fal, BFormula.imp⟩
 prefix:59 "∀ᵇ " => BFormula.all
 @[reducible] def BFormula.exists (p : BFormula 𝓛 (m + 1)) := ~ ∀ᵇ (~ p)
@@ -180,19 +189,19 @@ def BFormula.alls : ∀ {m}, BFormula 𝓛 m → Sentence 𝓛
 prefix:59 "∀* " => BFormula.alls
 
 def BFormula.unbounded : BFormula 𝓛 m → Formula 𝓛
-| p ⬝ₚ ts => p ⬝ₚ ts.unbounded
+| p ⬝ₚᵇ ts => p ⬝ₚ ts.unbounded
 | ⊥ => ⊥
 | p ⟶ q => p.unbounded ⟶ q.unbounded
 | ∀ᵇ p => ∀' p.unbounded
 
-@[simp] theorem BFormula.unbounded_atom : (p ⬝ₚ ts : BFormula 𝓛 m).unbounded = p ⬝ₚ ts.unbounded := rfl
+@[simp] theorem BFormula.unbounded_atom : (p ⬝ₚᵇ ts : BFormula 𝓛 m).unbounded = p ⬝ₚ ts.unbounded := rfl
 @[simp] theorem BFormula.unbounded_fal : (⊥ : BFormula 𝓛 m).unbounded = ⊥ := rfl
 @[simp] theorem BFormula.unbounded_imp : (p ⟶ q : BFormula 𝓛 m).unbounded = p.unbounded ⟶ q.unbounded := rfl
 @[simp] theorem BFormula.unbounded_neg : (~ p : BFormula 𝓛 m).unbounded = ~ p.unbounded := rfl
 @[simp] theorem BFormula.unbounded_all : (∀ᵇ p).unbounded = ∀' p.unbounded := rfl
 
--- instance : CoeOut (BFormula 𝓛 m) (Formula 𝓛) := ⟨BFormula.unbounded⟩
-instance : Coe (Sentence 𝓛) (Formula 𝓛) := ⟨BFormula.unbounded⟩
+instance : CoeOut (BFormula 𝓛 m) (Formula 𝓛) := ⟨BFormula.unbounded⟩
+instance (prio := prioHigh) : Coe (Sentence 𝓛) (Formula 𝓛) := ⟨BFormula.unbounded⟩
 
 @[simp] def Formula.bound : Formula 𝓛 → ℕ
 | _ ⬝ₚ ts => ts.bound
@@ -201,7 +210,7 @@ instance : Coe (Sentence 𝓛) (Formula 𝓛) := ⟨BFormula.unbounded⟩
 | ∀' p => p.bound - 1
 
 def Formula.bounded : (p : Formula 𝓛) → m ≥ p.bound → BFormula 𝓛 m
-| p ⬝ₚ ts, h => p ⬝ₚ ts.bounded h
+| p ⬝ₚ ts, h => p ⬝ₚᵇ ts.bounded h
 | ⊥, _ => ⊥
 | p ⟶ q, h => p.bounded (by simp at h; exact h.left) ⟶ q.bounded (by simp at h; exact h.right)
 | ∀' p, h => ∀ᵇ p.bounded (by simp at h; exact h)
@@ -215,24 +224,23 @@ theorem Formula.bounded_unbounded {p : Formula 𝓛} {h : m ≥ p.bound} :
   case all _ ih => simp [ih]
 
 def BFormula.subst : BFormula 𝓛 m → BSubst 𝓛 m k → BFormula 𝓛 k
-| p ⬝ₚ ts, σ => p ⬝ₚ ts[σ]ₜₛ
+| p ⬝ₚᵇ ts, σ => p ⬝ₚᵇ ts[σ]ₜₛᵇ
 | ⊥, _ => ⊥
 | p ⟶ q, σ => p.subst σ ⟶ q.subst σ
-| ∀ᵇ p, σ => ∀ᵇ (p.subst ⇑ₛσ)
+| ∀ᵇ p, σ => ∀ᵇ (p.subst ⇑ᵇσ)
 
-notation:80 p "[" σ "]ₚ" => BFormula.subst p σ
+notation:80 p "[" σ "]ₚᵇ" => BFormula.subst p σ
 
-@[simp] theorem BFormula.subst_atom {σ : BSubst 𝓛 m k} : (p ⬝ₚ ts)[σ]ₚ = p ⬝ₚ ts[σ]ₜₛ := rfl
-@[simp] theorem BFormula.subst_fal {σ : BSubst 𝓛 m k} : ⊥[σ]ₚ = ⊥ := rfl
-@[simp] theorem BFormula.subst_imp {σ : BSubst 𝓛 m k} : (p ⟶ q)[σ]ₚ = p[σ]ₚ ⟶ q[σ]ₚ := rfl
-@[simp] theorem BFormula.subst_neg {σ : BSubst 𝓛 m k} : (~ p)[σ]ₚ = ~ p[σ]ₚ := rfl
-@[simp] theorem BFormula.subst_all {σ : BSubst 𝓛 m k} : (∀ᵇ p)[σ]ₚ = ∀ᵇ p[⇑ₛσ]ₚ := rfl
+@[simp] theorem BFormula.subst_atom : (p ⬝ₚᵇ ts)[σ]ₚᵇ = p ⬝ₚᵇ ts[σ]ₜₛᵇ := rfl
+@[simp] theorem BFormula.subst_fal : ⊥[σ]ₚᵇ = ⊥ := rfl
+@[simp] theorem BFormula.subst_imp : (p ⟶ q)[σ]ₚᵇ = p[σ]ₚᵇ ⟶ q[σ]ₚᵇ := rfl
+@[simp] theorem BFormula.subst_neg : (~ p)[σ]ₚᵇ = ~ p[σ]ₚᵇ := rfl
+@[simp] theorem BFormula.subst_all : (∀ᵇ p)[σ]ₚᵇ = ∀ᵇ p[⇑ᵇσ]ₚᵇ := rfl
 
-def BFormula.shift (p : BFormula 𝓛 m) := p[BSubst.shift]ₚ
-prefix:max "↑ₚ" => BFormula.shift
+def BFormula.shift (p : BFormula 𝓛 m) := p[BSubst.shift]ₚᵇ
+prefix:max "↑ₚᵇ" => BFormula.shift
 
-theorem BFormula.subst_id {p : BFormula 𝓛 m} :
-  p[(idₛ : BSubst 𝓛 m m)]ₚ = p := by
+theorem BFormula.subst_id : p[idᵇ]ₚᵇ = p := by
   induction p <;> try simp
   case atom => simp [BTerms.subst_id]
   case fal => rfl
@@ -243,11 +251,11 @@ theorem BFormula.subst_id {p : BFormula 𝓛 m} :
     funext x
     cases x using Fin.cases
     · rfl
-    · simp [BSubst.lift, BSubst.id, BTerm.shift, BSubst.shift]
+    · simp [BSubst.lift, BSubst.cons, BSubst.id, BTerm.shift, BSubst.shift]
 
 theorem BFormula.unbounded_subst_eq
   {p : BFormula 𝓛 m} {σ : BSubst 𝓛 m k} {σ' : Subst 𝓛} :
-  (∀ x, (σ x).unbounded = σ' x) → p[σ]ₚ.unbounded = p.unbounded[σ']ₚ := by
+  (∀ x, σ x = σ' x) → p[σ]ₚᵇ = p[σ']ₚ := by
   intro h
   induction p generalizing k σ' <;> try simp
   case atom p ts => simp [BTerms.unbounded_subst_eq h]
@@ -258,32 +266,32 @@ theorem BFormula.unbounded_subst_eq
     intro x
     cases x using Fin.cases
     · rfl
-    · simp [BSubst.lift, Subst.lift, BTerm.unbounded_shift_eq, h]
+    · simp [BSubst.lift, BSubst.cons, Subst.lift, BTerm.unbounded_shift_eq, h]
 
 theorem Formula.bounded_subst_single_unbounded
   {p : Formula 𝓛} {h₁ : m + 1 ≥ p.bound}
   {t : Term 𝓛} {h₂ : m ≥ t.bound} :
-  (p.bounded h₁)[BSubst.single (t.bounded h₂)]ₚ.unbounded = p[↦ₛ t]ₚ := by
+  (p.bounded h₁)[↦ᵇ (t.bounded h₂)]ₚᵇ = p[↦ₛ t]ₚ := by
   conv => rhs; rw [←Formula.bounded_unbounded (h := h₁)]
   apply BFormula.unbounded_subst_eq
   intro x
   cases x using Fin.cases
-  · simp [BSubst.single, Subst.single, Term.bounded_unbounded]
-  · simp [BSubst.single, BSubst.id, Subst.single, Term.bounded_unbounded]
+  · simp [BSubst.single, BSubst.cons, Subst.single, Term.bounded_unbounded]
+  · simp [BSubst.single, BSubst.cons, BSubst.id, Subst.single, Term.bounded_unbounded]
 
-theorem Sentence.unbounded_subst_eq
-  {p : Sentence 𝓛} {σ : Subst 𝓛} : p[σ]ₚ = p := by
+theorem Sentence.unbounded_subst_eq {p : Sentence 𝓛} {σ : Subst 𝓛} :
+  p[σ]ₚ = p := by
   conv => rhs; rw [←BFormula.subst_id (p := p)]
   symm
   apply BFormula.unbounded_subst_eq
   apply finZeroElim
 
-theorem Sentence.shift_eq {p : Sentence 𝓛} : ↑ₚ(p : Formula 𝓛) = p :=
+theorem Sentence.shift_eq {p : Sentence 𝓛} :
+  ↑ₚp = (p : Formula 𝓛) :=
   Sentence.unbounded_subst_eq
 
-theorem Sentence.foralls_elim
-  {p : BFormula 𝓛 m} {σ : Subst 𝓛} :
-  Γ ⊢ ∀* p ⟶ p.unbounded[σ]ₚ := by
+theorem Sentence.foralls_elim {p : BFormula 𝓛 m} {σ : Subst 𝓛} :
+  Γ ⊢ ∀* p ⟶ p[σ]ₚ := by
   induction' m with m ih generalizing σ
   · rw [Sentence.unbounded_subst_eq]
     exact Proof.identity
@@ -299,7 +307,7 @@ theorem Sentence.foralls_elim
     apply Proof.forall_elim
 
 theorem Sentence.foralls_elim_self {p : BFormula 𝓛 m} :
-  Γ ⊢ ∀* p ⟶ p.unbounded := by
+  Γ ⊢ ∀* p ⟶ (p : Formula 𝓛) := by
   have h := Sentence.foralls_elim (Γ := Γ) (p := p) (σ := Subst.id)
   simp [Formula.subst_id] at h
   exact h
@@ -309,53 +317,53 @@ theorem Sentence.foralls_elim_self {p : BFormula 𝓛 m} :
 def BAssignment (𝓜 : Structure 𝓛) (m) := Fin m → 𝓜.𝓤
 
 def BAssignment.nil : BAssignment 𝓜 0 := finZeroElim
-notation "[]ₐ" => BAssignment.nil
+notation "[]ₐᵇ" => BAssignment.nil
 
 def BAssignment.cons (u : 𝓜.𝓤) (ρ : BAssignment 𝓜 m) : BAssignment 𝓜 (m + 1) := Fin.cons u ρ
-infixr:80 " ∷ₐ " => BAssignment.cons
+infixr:80 " ∷ₐᵇ " => BAssignment.cons
 
 def BAssignment.unbounded (ρ : BAssignment 𝓜 m) : Assignment 𝓜 :=
   λ x => if h : x < m then ρ ⟨x, h⟩ else default
 
 mutual
 @[simp] def BTerm.interp : BTerm 𝓛 m → (𝓜 : Structure 𝓛) → BAssignment 𝓜 m → 𝓜.𝓤
-| #'x, _, ρ => ρ x
-| f ⬝ₜ ts, 𝓜, ρ => 𝓜.𝓕 f (ts.interp 𝓜 ρ)
+| #ᵇx, _, ρ => ρ x
+| f ⬝ₜᵇ ts, 𝓜, ρ => 𝓜.𝓕 f (ts.interp 𝓜 ρ)
 @[simp] def BTerms.interp : BTerms 𝓛 m n → (𝓜 : Structure 𝓛) → BAssignment 𝓜 m → Vector 𝓜.𝓤 n
-| []ₜ, _, _ => []ᵥ
-| t ∷ₜ ts, 𝓜, ρ => t.interp 𝓜 ρ ∷ᵥ ts.interp 𝓜 ρ
+| []ₜᵇ, _, _ => []ᵥ
+| t ∷ₜᵇ ts, 𝓜, ρ => t.interp 𝓜 ρ ∷ᵥ ts.interp 𝓜 ρ
 end
 
-notation:80 "⟦" t "⟧ₜ " 𝓜 ", " ρ:80 => BTerm.interp t 𝓜 ρ
-notation:80 "⟦" ts "⟧ₜₛ " 𝓜 ", " ρ:80 => BTerms.interp ts 𝓜 ρ
+notation:80 "⟦" t "⟧ₜᵇ " 𝓜 ", " ρ:80 => BTerm.interp t 𝓜 ρ
+notation:80 "⟦" ts "⟧ₜₛᵇ " 𝓜 ", " ρ:80 => BTerms.interp ts 𝓜 ρ
 
 @[simp] def BFormula.interp : BFormula 𝓛 m → (𝓜 : Structure 𝓛) → BAssignment 𝓜 m → Prop
-| p ⬝ₚ ts, 𝓜, ρ => 𝓜.𝓟 p (⟦ ts ⟧ₜₛ 𝓜, ρ)
+| p ⬝ₚᵇ ts, 𝓜, ρ => 𝓜.𝓟 p (⟦ ts ⟧ₜₛᵇ 𝓜, ρ)
 | ⊥, _, _ => False
 | p ⟶ q, 𝓜, ρ => p.interp 𝓜 ρ → q.interp 𝓜 ρ
-| ∀ᵇ p, 𝓜, ρ => ∀ u, p.interp 𝓜 (u ∷ₐ ρ)
+| ∀ᵇ p, 𝓜, ρ => ∀ u, p.interp 𝓜 (u ∷ₐᵇ ρ)
 
-notation:80 "⟦" p "⟧ₚ" 𝓜 ", " ρ:80 => BFormula.interp p 𝓜 ρ
-notation:80 "⟦" p "⟧ₛ" 𝓜:80 => BFormula.interp p 𝓜 []ₐ
+notation:80 "⟦" p "⟧ₚᵇ" 𝓜 ", " ρ:80 => BFormula.interp p 𝓜 ρ
+notation:80 "⟦" p "⟧ₛᵇ" 𝓜:80 => BFormula.interp p 𝓜 []ₐᵇ
 
 mutual
 theorem BTerm.unbounded_interp_eq {ρ : BAssignment 𝓜 m} {ρ' : Assignment 𝓜} :
-  (∀ x, ρ x = ρ' x) → ⟦ t ⟧ₜ 𝓜, ρ = ⟦ t.unbounded ⟧ₜ 𝓜, ρ' :=
+  (∀ x, ρ x = ρ' x) → ⟦ t ⟧ₜᵇ 𝓜, ρ = ⟦ t ⟧ₜ 𝓜, ρ' :=
   match t with
-  | #'x => by intro h; simp [h]
-  | f ⬝ₜ ts => by intro h; simp; rw [BTerms.unbounded_interp_eq h]
+  | #ᵇx => by intro h; simp [h]
+  | f ⬝ₜᵇ ts => by intro h; simp; rw [BTerms.unbounded_interp_eq h]
 theorem BTerms.unbounded_interp_eq {ρ : BAssignment 𝓜 m} {ρ' : Assignment 𝓜} :
-  (∀ x, ρ x = ρ' x) → ⟦ ts ⟧ₜₛ 𝓜, ρ = ⟦ ts.unbounded ⟧ₜₛ 𝓜, ρ' :=
+  (∀ x, ρ x = ρ' x) → ⟦ ts ⟧ₜₛᵇ 𝓜, ρ = ⟦ ts ⟧ₜₛ 𝓜, ρ' :=
   match ts with
-  | []ₜ => by intro; rfl
-  | t ∷ₜ ts => by
+  | []ₜᵇ => by intro; rfl
+  | t ∷ₜᵇ ts => by
     intro h
     simp
     rw [BTerm.unbounded_interp_eq h, BTerms.unbounded_interp_eq h]
 end
 
 theorem BFormula.unbounded_interp_eq {ρ : BAssignment 𝓜 m} {ρ' : Assignment 𝓜} :
-  (∀ x, ρ x = ρ' x) → ⟦ p ⟧ₚ 𝓜, ρ = ⟦ p.unbounded ⟧ₚ 𝓜, ρ' := by
+  (∀ x, ρ x = ρ' x) → ⟦ p ⟧ₚᵇ 𝓜, ρ = ⟦ p ⟧ₚ 𝓜, ρ' := by
   intro h
   induction p generalizing ρ' <;> simp
   case atom => simp [BTerms.unbounded_interp_eq h]
@@ -370,21 +378,21 @@ theorem BFormula.unbounded_interp_eq {ρ : BAssignment 𝓜 m} {ρ' : Assignment
     · simp [BAssignment.cons, Assignment.cons]; apply h
 
 theorem Sentence.unbounded_interp_eq
-  {p : Sentence 𝓛} {ρ : Assignment 𝓜} : ⟦ p ⟧ₛ 𝓜 = ⟦ p ⟧ₚ 𝓜, ρ := by
+  {p : Sentence 𝓛} {ρ : Assignment 𝓜} : ⟦ p ⟧ₛᵇ 𝓜 = ⟦ p ⟧ₚ 𝓜, ρ := by
   apply BFormula.unbounded_interp_eq
   apply finZeroElim
 
 theorem BTerm.unbounded_interp {ρ : BAssignment 𝓜 m} :
-  ⟦ t ⟧ₜ 𝓜, ρ = ⟦ t.unbounded ⟧ₜ 𝓜, ρ.unbounded := by
+  ⟦ t ⟧ₜᵇ 𝓜, ρ = ⟦ t ⟧ₜ 𝓜, ρ.unbounded := by
   apply BTerm.unbounded_interp_eq
   intro ⟨x, h⟩; simp [BAssignment.unbounded, h]
 
 theorem BTerms.unbounded_interp {ρ : BAssignment 𝓜 m} :
-  ⟦ ts ⟧ₜₛ 𝓜, ρ = ⟦ ts.unbounded ⟧ₜₛ 𝓜, ρ.unbounded := by
+  ⟦ ts ⟧ₜₛᵇ 𝓜, ρ = ⟦ ts ⟧ₜₛ 𝓜, ρ.unbounded := by
   apply BTerms.unbounded_interp_eq
   intro ⟨x, h⟩; simp [BAssignment.unbounded, h]
 
 theorem BFormula.unbounded_interp {ρ : BAssignment 𝓜 m} :
-  ⟦ p ⟧ₚ 𝓜, ρ = ⟦ p.unbounded ⟧ₚ 𝓜, ρ.unbounded := by
+  ⟦ p ⟧ₚᵇ 𝓜, ρ = ⟦ p ⟧ₚ 𝓜, ρ.unbounded := by
   apply BFormula.unbounded_interp_eq
   intro ⟨x, h⟩; simp [BAssignment.unbounded, h]
