MathematicalLogic/FirstOrder/Theory.lean
@@ -1,18 +1,17 @@
 import MathematicalLogic.FirstOrder.Semantics
 import MathematicalLogic.FirstOrder.Bounded
 
-universe u
-
 @[reducible] def Theory (𝓛) := Set (Sentence 𝓛)
 
-def Theory.toContext (𝓣 : Theory 𝓛) : Context 𝓛 := {↑p | p ∈ 𝓣}
+def Theory.toContext (𝓣 : Theory 𝓛) : Context 𝓛 :=
+  { BFormula.unbounded p | p ∈ 𝓣 }
 
 def Theory.Proof (𝓣 : Theory 𝓛) (p : Formula 𝓛) := 𝓣.toContext ⊢ p
 
 infix:50 " ⊢ " => Theory.Proof
 
 theorem Theory.axioms {p : Sentence 𝓛} {𝓣 : Theory 𝓛} :
-  p ∈ 𝓣 → 𝓣 ⊢ ↑p := by
+  p ∈ 𝓣 → 𝓣 ⊢ (p : Formula 𝓛) := by
   intro h
   apply Proof.assumption
   exists p
@@ -21,7 +20,7 @@ lemma Theory.shift_eq {𝓣 : Theory 𝓛} : ↑ₚₛ𝓣.toContext = 𝓣.toCo
   unfold Theory.toContext
   simp [Context.lift, Sentence.shift_eq]
 
-theorem Theory.generalization {𝓣 : Theory 𝓛} :
+theorem Theory.generalization {𝓣 : Theory 𝓛} {p : Formula 𝓛} :
   𝓣 ⊢ p → 𝓣 ⊢ ∀' p := by
   intro h
   apply Proof.generalization
@@ -29,7 +28,7 @@ theorem Theory.generalization {𝓣 : Theory 𝓛} :
   exact h
 
 def Model (𝓣 : Theory 𝓛) : Type (u + 1) :=
-  { 𝓜 : Structure 𝓛 | ∀ p ∈ 𝓣, ⟦ p ⟧ₛ 𝓜 }
+  { 𝓜 : Structure 𝓛 | ∀ p ∈ 𝓣, ⟦ p ⟧ₛᵇ 𝓜 }
 
 namespace Model
 
@@ -44,13 +43,12 @@ instance : CoeOut (Model 𝓣) (Structure 𝓛) where
 
 end Model
 
-theorem Theory.soundness
-  {𝓣 : Theory 𝓛} {𝓜 : Model 𝓣} {ρ : Assignment 𝓜} :
+theorem Theory.soundness {𝓣 : Theory 𝓛} {p : Formula 𝓛} {𝓜 : Model 𝓣} {ρ : Assignment 𝓜} :
   𝓣 ⊢ p → ⟦ p ⟧ₚ 𝓜, ρ := by
-  rintro h
+  intro h
   apply _root_.soundness
   · exact h
-  · rintro q ⟨p, h₁, h₂⟩
+  · intro q ⟨p, h₁, h₂⟩
     subst h₂
     simp [←Sentence.unbounded_interp_eq]
     apply 𝓜.property
